benign example

Dafny/examples/simpleBenign/BenignCode.s.dfy
@@ -5,7 +5,7 @@ include "../../LLVM/behaviorLemmas.i.dfy"
 include "../../Libraries/Seqs.s.dfy"
 include "../../LLVM/memory.i.dfy"
 
-module challenge6Code{
+module simpleBenignCode{
     import opened control_flow
     import opened LLVM_defRE
     import opened types
@@ -13,13 +13,28 @@ module challenge6Code{
     import opened behavior_lemmas
     import opened memory
 
+    predicate validStartingState(s:state)
+    {
+        var var_z := LV(" var_z ");
+        var var_cmp := LV(" var_cmp ");
+        var var_cmp1 := LV(" var_cmp1 ");
+        var var_add := LV(" var_add ");
+        var var_cmp2 := LV(" var_cmp2 ");
+        var var_0 := LV(" var_0 ");
 
-    function challenge_7_transport_handler_code(var_x:operand):codeRe
+        && "var_z" in s.lvs
+        && "var_cmp" in s.lvs
+        && "var_cmp1" in s.lvs
+        && "var_add" in s.lvs
+        && "var_cmp2" in s.lvs
+        && "var_0" in s.lvs
+    }
+
+    function benign_patch_code(var_x:operand):codeRe
     {
 
         var var_z := LV(" var_z ");
         var var_cmp := LV(" var_cmp ");
-        //var var_x := LV(" var_x ");
         var var_cmp1 := LV(" var_cmp1 ");
         var var_add := LV(" var_add ");
         var var_cmp2 := LV(" var_cmp2 ");
@@ -27,9 +42,11 @@ module challenge6Code{
 
         var return_ := Block([Ins(RET(D(Void)))]);
 
-        var if_end4 := Block([Ins(UNCONDBR(return_))]);
+        var if_end4 := Block([Ins(CALL(D(Void),[printf_code(global_str1())])),
+        Ins(UNCONDBR(return_))]);
 
-        var if_then3 := Block([Ins(UNCONDBR(if_end4))]);
+        var if_then3 := Block([Ins(CALL(D(Void),[printf_code(global_str())])),
+        Ins(UNCONDBR(if_end4))]);
 
         var if_end := Block([Ins(ADD(var_add,4,var_x,D(Int(2147483646,IntType(4,false))))),
         Ins(STORE(var_add,var_z)),
@@ -46,6 +63,101 @@ module challenge6Code{
         Ins(BR(var_x,if_then,lor_lhs_false))]);
 
         entry
+    }
+
+    function benign_vuln_code(var_x:operand):codeRe
+    {
+
+        var var_z := LV(" var_z ");
+        var var_cmp := LV(" var_cmp ");
+        var var_cmp1 := LV(" var_cmp1 ");
+        var var_add := LV(" var_add ");
+        var var_cmp2 := LV(" var_cmp2 ");
+        var var_0 := LV(" var_0 ");
+
+        var return_ := Block([Ins(RET(D(Void)))]);
+
+        var if_end4 := Block([Ins(CALL(D(Void),[printf_code(global_str1())])),
+        Ins(UNCONDBR(return_))]);
+
+        var if_then3 := Block([Ins(CALL(D(Void),[printf_code(global_str())])),
+        Ins(UNCONDBR(if_end4))]);
+
+        var if_end := Block([Ins(ADD(var_add,4,var_x,D(Int(2147483646,IntType(4,false))))),
+        Ins(STORE(var_add,var_z)),
+        Ins(ICMP(var_cmp2,sgt,4,var_add,D(Int(0,IntType(4,false))))),
+        Ins(BR(var_cmp2,if_then3,if_end4))]);
+
+        var if_then := Block([Ins(UNCONDBR(return_))]);
+
+        var lor_lhs_false := Block([Ins(ICMP(var_cmp1,sgt,4,var_x,D(Int(2,IntType(4,false))))),
+        Ins(BR(var_x,if_then,if_end))]);
+
+        var entry := Block([Ins(ALLOCA(var_z,4)),
+        Ins(ICMP(var_cmp,slt,4,var_x,D(Int(0,IntType(4,false))))),
+        Ins(BR(var_x,if_then,lor_lhs_false))]);
+
+        entry
+    }
+
+    function benign_patch_SOI(s:state):codeRe
+        requires SOI_ASSIMPTIONS(s)
+    {
+
+        var var_cmp2 := LV(" var_cmp2 ");
+        var var_0:operand :| var_0.LV? && var_0.l in s.lvs && var_0.l == "var_0";
+
+        var return_ := Block([Ins(RET(D(Void)))]);
+
+        var if_end4 := Block([Ins(CALL(D(Void),[printf_code(global_str1())])),
+        Ins(UNCONDBR(return_))]);
+
+        var if_then3 := Block([Ins(CALL(D(Void),[printf_code(global_str())])),
+        Ins(UNCONDBR(if_end4))]);
+
+        var if_end := Block([
+        Ins(ICMP(var_cmp2,ugt,4,var_0,D(Int(0,IntType(4,false))))),
+        Ins(BR(var_cmp2,if_then3,if_end4))]);
+
+        if_end
+
+        // ASSUMPTIONS (ENGLISH)
+        // var_0 has the value of x :: MAX_INT-1 >= x && x < MAX_INT+1
+    }
+
+    predicate SOI_ASSIMPTIONS(s:state)
+    {
+        var var_0 := LV("var_0");
+        ValidState(s)
+        && ValidOperand(s,var_0)
+        && s.lvs["var_0"].Int?
+        && s.lvs["var_0"].val >= 2147483646
+        && s.lvs["var_0"].val < 2147483648
+        && s.lvs["var_0"].itype.size == 4
+    }
+
+
+
+
+    function global_str():Data
+    {
+       // "z is positive" 
+        var str:Bytes := [0x7a, 0x20, 0x69, 0x73, 0x20, 0x70, 0x6f, 0x73, 0x69, 0x74, 0x69, 0x76, 0x65];
+        Bytes(str)
+    }
+
+    function global_str1():Data
+    {
+       // "done" 
+        var str1:Bytes := [0x64, 0x6f, 0x6e, 0x65];
+        Bytes(str1)
+    }
+
+
+
+    function printf_code(o:Data):codeRe
+    {
+        Block([Ins(VISIBLE_OUT(Out(o)))])
     }
 
 }
