Dafny/examples/Challenge7/Challenge7Code.s.dfy
@@ -17,87 +17,29 @@ module challenge7Code{
     function challenge_7_transport_handler_code_vuln():codeRe
     {
 
-        var var_read_frame_sroa_4122_8_extract_trunc := LV(" var_read_frame_sroa_4122_8_extract_trunc ");
-        var var_read_frame_coerce1 := LV(" var_read_frame_coerce1 ");
-        var var_read_frame_sroa_8_8_extract_shift := LV(" var_read_frame_sroa_8_8_extract_shift ");
-        var var_read_frame_sroa_8_8_extract_trunc := LV(" var_read_frame_sroa_8_8_extract_trunc ");
-        var var_read_frame_sroa_10_8_extract_shift := LV(" var_read_frame_sroa_10_8_extract_shift ");
-        var var_read_frame_sroa_10_8_extract_trunc := LV(" var_read_frame_sroa_10_8_extract_trunc ");
-        var var_read_frame_sroa_11_8_extract_shift := LV(" var_read_frame_sroa_11_8_extract_shift ");
-        var var_read_frame_sroa_11_8_extract_trunc := LV(" var_read_frame_sroa_11_8_extract_trunc ");
-        var var_read_frame_sroa_12_8_extract_shift := LV(" var_read_frame_sroa_12_8_extract_shift ");
-        var var_read_frame_sroa_12_8_extract_trunc := LV(" var_read_frame_sroa_12_8_extract_trunc ");
-        var var_conv := LV(" var_conv ");
-        var var_read_frame_coerce0 := LV(" var_read_frame_coerce0 ");
-        var var_src := LV(" var_src ");
-        var var_and2126 := LV(" var_and2126 ");
-        var var_0 := LV(" var_0 ");
-        var var_cmp := LV(" var_cmp ");
-        var var_current_sa := LV(" var_current_sa ");
-        var var_read_frame_sroa_0_0_extract_trunc := LV(" var_read_frame_sroa_0_0_extract_trunc ");
-        var var_and6 := LV(" var_and6 ");
-        var var_Pivot := LV(" var_Pivot ");
-        var var_SwitchLeaf2 := LV(" var_SwitchLeaf2 ");
-        var var_SwitchLeaf := LV(" var_SwitchLeaf ");
-        var var_Pivot9 := LV(" var_Pivot9 ");
-        var var_SwitchLeaf7 := LV(" var_SwitchLeaf7 ");
-        var var_SwitchLeaf5 := LV(" var_SwitchLeaf5 ");
 
+var var_20 := LV(" var_20 ");
+var var_read_frame_coerce1 := LV(" var_read_frame_coerce1 ");
+var var_conv78 := LV(" var_conv78 ");
+var var_num_packets88 := LV(" var_num_packets88 ");
+var var_23 := LV(" var_23 ");
+var var_conv89 := LV(" var_conv89 ");
+var var_cmp90 := LV(" var_cmp90 ");
 
+var if_end93 := Block([Ins(RET(D(Void)))]);
 
-        var if_end111 := Block([Ins(RET(D(Void)))]);
+var if_end122 := Block([Ins(RET(D(Void)))]);
 
-        var sw_bb54 := Block([Ins(UNCONDBR(if_end111))]);
+var if_then92 := Block([Ins(UNCONDBR(if_end122))]);
 
-        var sw_bb45 := Block([Ins(UNCONDBR(if_end111))]);
+var entry := Block([Ins(TRUNC(var_20,8,var_read_frame_coerce1,4)),
+Ins(AND(var_conv78,var_20,D(Int(255,IntType(4,false))))),
+Ins(LOAD(var_23,1,var_num_packets88)),
+Ins(ZEXT(var_conv89,4,var_23,4)),
+Ins(ICMP(var_cmp90,ugt,4,var_conv78,var_conv89)),
+Ins(BR(var_conv78,if_then92,if_end93))]);
 
-        var if_else := Block([Ins(UNCONDBR(if_end111))]);
-
-        var NewDefault3 := Block([Ins(UNCONDBR(if_end111))]);
-
-        var NewDefault := Block([Ins(UNCONDBR(if_end111))]);
-
-        var LeafBlock4 := Block([Ins(ICMP(var_SwitchLeaf5,eq,1,var_read_frame_sroa_4122_8_extract_trunc,D(Int(16,IntType(1,false))))),
-        Ins(BR(var_read_frame_sroa_4122_8_extract_trunc,if_else,NewDefault3))]);
-
-        var LeafBlock6 := Block([Ins(ICMP(var_SwitchLeaf7,eq,1,var_read_frame_sroa_4122_8_extract_trunc,D(Int(19,IntType(1,false))))),
-        Ins(BR(var_read_frame_sroa_4122_8_extract_trunc,sw_bb45,NewDefault3))]);
-
-        var NodeBlock8 := Block([Ins(ICMP(var_Pivot9,slt,1,var_read_frame_sroa_4122_8_extract_trunc,D(Int(19,IntType(1,false))))),
-        Ins(BR(var_read_frame_sroa_4122_8_extract_trunc,LeafBlock4,LeafBlock6))]);
-
-        var sw_bb := Block([Ins(UNCONDBR(NodeBlock8))]);
-
-        var LeafBlock := Block([Ins(ICMP(var_SwitchLeaf,eq,4,var_and6,D(Int(15400960,IntType(4,false))))),
-        Ins(BR(var_and6,sw_bb54,NewDefault))]);
-
-        var LeafBlock1 := Block([Ins(ICMP(var_SwitchLeaf2,eq,4,var_and6,D(Int(15466496,IntType(4,false))))),
-        Ins(BR(var_and6,sw_bb,NewDefault))]);
-
-        var NodeBlock := Block([Ins(ICMP(var_Pivot,slt,4,var_and6,D(Int(15466496,IntType(4,false))))),
-        Ins(BR(var_and6,LeafBlock,LeafBlock1))]);
-
-        var if_then := Block([Ins(TRUNC(var_read_frame_sroa_0_0_extract_trunc,8,var_read_frame_coerce0,4)),
-        Ins(AND(var_and6,var_read_frame_sroa_0_0_extract_trunc,D(Int(16711680,IntType(4,false))))),
-        Ins(UNCONDBR(NodeBlock))]);
-
-        var entry := Block([Ins(TRUNC(var_read_frame_sroa_4122_8_extract_trunc,8,var_read_frame_coerce1,1)),
-        Ins(LSHR(var_read_frame_sroa_8_8_extract_shift,var_read_frame_coerce1,D(Int(8,IntType(8,false))))),
-        Ins(TRUNC(var_read_frame_sroa_8_8_extract_trunc,8,var_read_frame_sroa_8_8_extract_shift,2)),
-        Ins(LSHR(var_read_frame_sroa_10_8_extract_shift,var_read_frame_coerce1,D(Int(24,IntType(8,false))))),
-        Ins(TRUNC(var_read_frame_sroa_10_8_extract_trunc,8,var_read_frame_sroa_10_8_extract_shift,1)),
-        Ins(LSHR(var_read_frame_sroa_11_8_extract_shift,var_read_frame_coerce1,D(Int(32,IntType(8,false))))),
-        Ins(TRUNC(var_read_frame_sroa_11_8_extract_trunc,8,var_read_frame_sroa_11_8_extract_shift,1)),
-        Ins(LSHR(var_read_frame_sroa_12_8_extract_shift,var_read_frame_coerce1,D(Int(40,IntType(8,false))))),
-        Ins(TRUNC(var_read_frame_sroa_12_8_extract_trunc,8,var_read_frame_sroa_12_8_extract_shift,4)),
-        Ins(TRUNC(var_conv,8,var_read_frame_coerce0,1)),
-        Ins(STORE(var_conv,var_src)),
-        Ins(LSHR(var_and2126,var_read_frame_coerce0,D(Int(8,IntType(8,false))))),
-        Ins(TRUNC(var_0,8,var_and2126,1)),
-        Ins(ICMP(var_cmp,eq,1,var_0,var_current_sa)),
-        Ins(BR(var_0,if_then,if_end111))]);
-
-        entry
+entry
     }
 
        function challenge_7_transport_handler_code_patch():codeRe
