Dafny/examples/simpleBenign/simpleBenignProperties.i.dfy
@@ -1,0 +1,99 @@
+include "BenignCode.s.dfy"
+include "../../LLVM/behaviorLemmas.i.dfy"
+include "../../LLVM/llvmREFACTOR.i.dfy"
+include "../../LLVM/types.dfy"
+include "../../Libraries/Sets.i.dfy"
+
+module simpleBenignProperties{
+    import opened simpleBenignCode
+    import opened behavior_lemmas
+    import opened LLVM_defRE
+    import opened types
+    import opened Collections__Sets_i
+
+    //PATCH PROPERTIES
+
+    // benignPatch: "The patch does not add any NEW behaviors"
+    predicate benignPatch(pre:set<behavior>,post:set<behavior>)
+    {
+        var preOutput := allBehaviorOutputSet(pre);
+        var postOutput := allBehaviorOutputSet(post);
+        forall postB :: postB in postOutput ==> postB in preOutput
+    }
+
+    // successfulPatch: "The patch prunes the BAD (defined by MiniSpec) behaviors"
+    predicate successfulPatch(post:set<behavior>)
+    {
+        forall postB :: MiniSpec(postB) ==> !(postB in post)
+    }
+
+    // completePatch: "The patch preserves the GOOD behavior" // Name; complete -> preserving ? 
+    predicate completePatchMS(pre:set<behavior>,post:set<behavior>)
+    {
+        // forall p :: (p in a && !MiniSpec(p)) ==> p in b
+        var preModMs := MakeSubset(pre, x => !MiniSpec(x));
+        var preModMsOut := allBehaviorOutputSet(preModMs);
+        var postOutput := allBehaviorOutputSet(post);
+        forall preB :: behaviorOutput(preB) in preModMsOut ==> behaviorOutput(preB) in postOutput
+    }
+
+    predicate safePatchMS(pre:set<behavior>,post:set<behavior>)
+    {           
+    //  forall p :: (p in a && !MiniSpec(p)) <==> p in b
+        var preModMs := MakeSubset(pre, x => !MiniSpec(x));
+        var preModMsOut := allBehaviorOutputSet(preModMs);
+        var postOutput := allBehaviorOutputSet(post);
+        forall preB :: behaviorOutput(preB) in preModMsOut <==> behaviorOutput(preB) in postOutput
+    } 
+
+    // Describes/Excludes 'bad' behaviors in the Unpatched Code (ie preBehaviors)
+    predicate RemovedBehaviors(b:behavior)
+    {
+        true
+    }
+
+    predicate MiniSpec(b:behavior)
+    {
+        RemovedBehaviors(b)
+    }
+
+
+    // PROOF  
+
+    lemma patchIsBenign(s:state,vulnBehaviors:set<behavior>,patchBehaviors:set<behavior>)
+        requires nonTrivialBehaviorPreconditions(s,vulnBehaviors,patchBehaviors)
+        //ensures benignPatch(vulnBehaviors,patchBehaviors)
+    {
+    }
+
+    lemma patchIsSuccesful(s:state,vulnBehaviors:set<behavior>,patchBehaviors:set<behavior>)
+    requires nonTrivialBehaviorPreconditions(s,vulnBehaviors,patchBehaviors)
+    //ensures successfulPatch(patchBehaviors)
+    {
+    }
+    
+    lemma patchIsComplete(s:state,vulnBehaviors:set<behavior>,patchBehaviors:set<behavior>)
+    requires nonTrivialBehaviorPreconditions(s,vulnBehaviors,patchBehaviors)
+    //ensures completePatchMS(patchBehaviors)
+    {
+    }
+
+    // FINAL PROOF
+    lemma fullPatch(pre:set<behavior>,post:set<behavior>)
+        requires benignPatch(pre,post);
+        requires successfulPatch(post);
+        requires completePatchMS(pre,post);
+        //ensures safePatchMS(pre,post);
+    {
+    }
+
+  // UTILITY PREDICATE/LEMMAS
+   predicate nonTrivialBehaviorPreconditions(s:state,vulnBehaviors:set<behavior>,patchBehaviors:set<behavior>)
+    {
+        && ValidState(s)
+    }
+
+        
+
+
+}
