Dafny/examples/simpleBenign/simpleBenignisBenign.i.dfy
@@ -1,0 +1,48 @@
+include "BenignCode.s.dfy"
+include "../../LLVM/llvmREFACTOR.i.dfy"
+include "../../LLVM/types.dfy"
+include "../../Libraries/Seqs.s.dfy"
+
+module simpleBenignIsBenign{
+    import opened simpleBenignCode
+    import opened LLVM_defRE
+    import opened types
+    import opened Collections__Seqs_s
+
+
+    lemma unwrapPatchBehaviors(s:state, input:operand) returns (b:behavior) 
+        requires ValidState(s);
+        requires validStartingState(s);
+    {
+        var var_z := LV(" var_z ");
+        var var_cmp := LV(" var_cmp ");
+        var var_cmp1 := LV(" var_cmp1 ");
+        var var_add := LV(" var_add ");
+        var var_cmp2 := LV(" var_cmp2 ");
+        var var_0 := LV(" var_0 ");
+    
+        //reveal_BehaviorEvalsCode();
+        var c := benign_patch_code(input);
+
+        assert |c.block| == 3;
+
+        b := [s] + evalCodeRE(c,s);
+        var step,remainder,subBehavior := unwrapBlockWitness(b,c.block,s);
+
+        step,remainder,subBehavior := unwrapBlockWitness(subBehavior,remainder,last(step));
+            
+
+        //var var_z:LV := s.lvs["var_z"];
+
+        assert b[0] == s;
+        assert "var_z" in s.lvs;
+        assert c.block[0] == Ins(ALLOCA(var_z,4));
+        //
+        assert b[1] == evalInsRe(ALLOCA(var_z,4),s);
+        assert ValidInstruction(s,ALLOCA(var_z,4));
+        assert StateNext(b[0],b[1]);
+        //assert ValidOperand(b[1],call);
+
+
+    }
+}
